theories/rules/rules_Get.v
@@ -197,7 +197,7 @@ Section cap_lang_rules.
     iApply (wp2_opt_incrementPC with "[$Hσ Hpc_a Hφ]").
     { rewrite dom_insert. apply elem_of_union_r. now rewrite elem_of_dom HPC. }
     iSplit.
-    - iIntros (φt' lrt') "Hσ %Hlin %Hin".
+    - iIntros "Hσ %Hlin %Hin".
       iDestruct (state_interp_transient_elim_abort with "Hσ") as "(Hσ & Hregs & _)".
       iFrame.
       iApply ("Hφ" with "[$Hpc_a $Hregs]").
