theories/rules/rules_IsUnique.v
@@ -240,7 +240,7 @@ Section cap_lang_rules.
     state_interp_transient σ σt lreg lrt lmem lmt ⊢
     ⌜ unique_in_registersL lreg src lwsrc ⌝.
   Proof.
-    iIntros (Hsweep Hsrc) "(((Hσ & Hregs & Hmem) & Hcommit) & _)".
+    iIntros (Hsweep Hsrc) "((Hσ & Hregs & Hmem) & Hcommit)".
     iDestruct "Hσ" as (lr lm vmap) "(Hr & Hm & %HLinv)"; simpl in HLinv.
     iDestruct (gen_heap_valid_inclSepM with "Hr Hregs") as "%Hregs_incl".
     iPureIntro.
@@ -326,22 +326,18 @@ Section cap_lang_rules.
   (* TODO lemma à la update_state_interp_from_mem_mod ,
        i.e. that updates the actual state *)
   Lemma update_state_interp_next_version
-    {σ Ep lregs lmem src lwsrc p b e a v} :
+    {σ lregs lmem src lwsrc p b e a v} :
 
     sweep (mem σ) (reg σ) src = true ->
     lregs !! src = Some lwsrc ->
     get_lcap lwsrc = Some (LSCap p b e a v) ->
 
-    state_interp_logical σ
-    ∗ ([∗ map] k↦y ∈ lregs, k ↦ᵣ y)
-    ∗ ([∗ map] la↦dw ∈ (full_own_mem lmem), la ↦ₐ{dw.1} dw.2)
-    ⊢ |={Ep}=>
+    state_interp_with_res σ lregs (full_own_mem lmem)
+    ⊢ |==>
           ∃ glm, ⌜ lmem ⊆ glm ⌝ ∗
           let lmem' := update_version_region glm (finz.seq_between b e) v lmem in
           ⌜ is_valid_updated_lmemory glm lmem (finz.seq_between b e) v lmem'⌝ ∗
-          state_interp_logical σ
-          ∗ ([∗ map] k↦y ∈ (<[src:=next_version_lword lwsrc]> lregs), k ↦ᵣ y)
-          ∗ ([∗ map] la↦dw ∈ (full_own_mem lmem'), la ↦ₐ{dw.1} dw.2).
+            state_interp_with_res σ (<[src:=next_version_lword lwsrc]> lregs) (full_own_mem lmem').
   Proof.
     iIntros (Hsweep Hlsrc Hlcap_wsrc) "(Hσ & Hregs & Hmem)".
     iDestruct "Hσ" as (lr lm vmap) "(Hr & Hm & %HLinv)"; simpl in HLinv.
@@ -399,6 +395,68 @@ Section cap_lang_rules.
     now iApply map_full_own.
   Qed.
 
+  Lemma update_state_interp_with_res_next_version {σt lregt lmemt src lwsrc p b e a v}:
+    sweep (mem σt) (reg σt) src = true ->
+    lregt !! src = Some lwsrc ->
+    get_lcap lwsrc = Some (LSCap p b e a v) ->
+    state_interp_with_res σt lregt (full_own_mem lmemt) ⊢
+      |==> (∃ glm,
+          ⌜ lmemt ⊆ glm ⌝ ∗
+          let lmemt' : LMem := update_version_region glm (finz.seq_between b e) v lmemt in
+          let lregt' : LReg := <[src:=next_version_lword lwsrc]> lregt in
+          ⌜ is_valid_updated_lmemory glm lmemt (finz.seq_between b e) v lmemt'⌝ ∗
+          (* remove the following pure fact and move into separate lemma *)
+          ∃ lreg_t lmem_t cur_map,
+            ⌜ lregt' ⊆ lreg_t ⌝
+            ∗ ⌜ lmemt' ⊆ lmem_t ⌝ ∗
+            ⌜state_phys_log_corresponds σt.(reg) σt.(mem) lreg_t lmem_t cur_map⌝ ∗
+            state_interp_with_res σt lregt' (full_own_mem lmemt')).
+  Proof.
+    iIntros (Hsweep Hsrc Hcap_lwsrc) "Hσrm".
+    iDestruct (state_interp_corr with "Hσrm") as "%Hcor".
+    destruct Hcor as (lrt & lmt & vmap & Hlregt_incl & Hlmemt_incl & HLinv).
+    rewrite snd_fmap_pair_inv in Hlmemt_incl.
+    assert (HNoDup : NoDup (finz.seq_between b e)) by (apply finz_seq_between_NoDup).
+    assert (lrt !! src = Some lwsrc) as Hsrc' by (eapply lookup_weaken in Hsrc ; eauto).
+    opose proof (sweep_true_specL _ _ _ _ _ _ _ _ _ Hsweep) as Hsweep'; eauto.
+    iDestruct (update_state_interp_next_version  with "Hσrm") as "H"
+    ; eauto.
+    iMod "H".
+    iModIntro.
+    iDestruct "H" as (glm) "(%Hincl & %Hvalid & Hσ & Hlr & Hlm)".
+
+    set (lmemt' := update_version_region glm (finz.seq_between b e) v lmemt).
+    set (lmt' := update_version_region glm (finz.seq_between b e) v lmt).
+    set (vmap' := update_version_region_vmap (finz.seq_between b e) v vmap).
+
+    iExists glm.
+    iFrame.
+    iSplit ; first done.
+    iSplit ; first done.
+
+    iPureIntro; cbn.
+    exists (<[src:=next_version_lword lwsrc]> lrt), lmemt', vmap'.
+    split; [|split; [|split] ]; auto.
+
+    { by apply insert_mono. }
+    {
+      eapply update_version_region_lreg_corresponds_src'; eauto.
+      eapply update_version_word_region_update_lword; eauto.
+      eapply lreg_corresponds_read_iscur; eauto.
+      by destruct HLinv.
+    }
+    {
+      subst lmt' vmap' lmemt'.
+      destruct HLinv as (HLinvreg & HLinvmem).
+      eapply update_version_region_preserves_mem_corresponds; eauto.
+      admit.
+      admit.
+      admit.
+      admit.
+      admit.
+    }
+  Admitted.
+
   Lemma update_state_interp_transient_next_version {σ σt lreg lregt lmem lmemt src lwsrc p b e a v}:
     sweep (mem σt) (reg σt) src = true ->
     lregt !! src = Some lwsrc ->
@@ -420,11 +478,9 @@ Section cap_lang_rules.
             ⌜ lregt' ⊆ lreg_t ⌝
             ∗ ⌜ snd <$> (full_own_mem lmemt') ⊆ lmem_t ⌝ ∗
             ⌜state_phys_log_corresponds σt.(reg) σt.(mem) lreg_t lmem_t cur_map⌝ ∗
-            state_interp_logical σt
-            ∗ ([∗ map] k↦y ∈ lregt', k ↦ᵣ y)
-            ∗ ([∗ map] k↦y ∈ (full_own_mem lmemt'), k ↦ₐ{y.1} y.2)).
+            state_interp_with_res σt lregt' (full_own_mem lmemt')).
   Proof.
-    iIntros (Hsweep Hsrc Hcap_lwsrc) "(((Hσ & Hregs & Hmem) & Hcommit) & %Hcor)".
+    iIntros (Hsweep Hsrc Hcap_lwsrc) "((Hσ & Hregs & Hmem) & Hcommit)".
     cbn in *.
     destruct Hcor as (lrt & lmt & vmap & Hlregt_incl & Hlmemt_incl & HLinv).
     rewrite snd_fmap_pair_inv in Hlmemt_incl.
@@ -546,7 +602,7 @@ Section cap_lang_rules.
         }
         iSplit.
         { (* failure case: incrementing the pc failed *)
-          iIntros (ec lregs') "Hσ %Hlincr %Hincr".
+          iIntros "Hσ %Hlincr %Hincr".
           iDestruct (state_interp_transient_elim_abort with "Hσ") as "($ & Hregs & Hmem)".
           rewrite big_sepM_fmap.
           iApply ("Hφ" with "[$Hregs $Hmem]").
@@ -572,23 +628,31 @@ Section cap_lang_rules.
         all: eapply IsUnique_success_true_is_sealed; eauto.
 
 
-      + iDestruct (update_state_interp_transient_next_version with "Hσ") as "Hσ" ; eauto.
-        change (<[dst:=WInt 1]> (reg σ)) with (reg (update_reg σ dst (WInt 1))).
+      + change (<[dst:=WInt 1]> (reg σ)) with (reg (update_reg σ dst (WInt 1))).
         iApply (wp2_opt_incrementPC with "[Hσ Hφ]").
         { pose proof (elem_of_dom_2 _ _ _ HPC).
-          now set_solver.}
-        unfold state_interp_transient.
+          now set_solver. }
         iSplitR "Hφ".
-        * admit.
+        * iSplitL "Hσ".
+          iDestruct "Hσ" as "[Hσ Hsplc]".
+          iApply (transiently_mono_2 with "[$Hσ]").
+          iIntros (Ep') "(Hσ & Hlregs & Hlmem)".
+          iMod (update_state_interp_transient_next_version with "Hσ") as "H".
+          assert (dst ∈ dom (<[src:=next_version_lword srcv]> lregs)) as Hdst
+            by (cbn in Dregs; set_solver).
+          iMod (update_state_interp_int Hdst with "[$Hσ $Hlregs]") as "[$ $]".
+          iModIntro.
+          iExact "Hlmem".
+          admit.
         * iSplit.
-          -- iIntros (ϕt' lrt') "[Hσ %Hσpure] %HincLPC %HincPC".
+          -- iIntros "[Hσ %Hσpure] %HincLPC %HincPC".
              iDestruct (transiently_abort with "Hσ") as "($ & Hlr' & Hlm')".
              iApply ("Hφ" with "[$Hlr' Hlm']").
              iSplitR.
              iPureIntro; constructor; try reflexivity.
              eapply IsUnique_fail_invalid_PC_upd; now eauto.
              admit.
-          -- iIntros (lrt' rs') "[Hσ %Hσpure] %HincLPC %HincPC".
+          -- iIntros "[Hσ %Hσpure] %HincLPC %HincPC".
              iApply wp2_val.
              iMod (transiently_commit with "Hσ") as "(Hσ & Hlrt' & Hlmt')".
              iModIntro.
@@ -604,7 +668,7 @@ Section cap_lang_rules.
              admit.
              admit.
     - iApply wp2_reg_lookup.
-      {cbn in Dregs; set_solver.}
+      {cbn in Dregs; set_solver. }
       iMod (state_interp_transient_intro_nodfracs (lm := lmem) with "[$Hregs $Hσ Hmem Hpca]") as "Hσ".
       { (* TODO: lemma! *)
         iCombine "Hpca Hmem" as "Hmem".
@@ -632,7 +696,7 @@ Section cap_lang_rules.
         iApply wp_opt2_eqn_both.
         iApply wp2_opt_incrementPC.
         { pose proof (elem_of_dom_2 _ _ _ HPC).
-          now set_solver.}
+          now set_solver. }
         unfold state_interp_transient.
         iSplitR "Hφ".
         * admit.
